src/examples/GPU.MatMulTile.fst
@@ -1,0 +1,163 @@
+module GPU.MatMulTile
+#lang-pulse
+
+#push-options "--fuel 1 --ifuel 1"
+
+open GPU
+
+module A    = Pulse.Lib.Array
+module SZ   = FStar.SizeT
+module Defs = GPU.MatMul.Defs
+module Kernel = GPU.MatMulTile.Kernel
+module Barrier = GPU.MatMulTile.Barrier
+
+ghost
+fn setup
+  (nblk: sz { nblk == SZ.(Kernel.rows_tile *^ Kernel.columns_tile) })
+  (nthr: sz { nthr == SZ.(Kernel.bdim *^ Kernel.bdim) })
+  (ga1 : gpu_array u64 (Kernel.rows * Kernel.shared))
+  (ga2 : gpu_array u64 (Kernel.shared * Kernel.columns))
+  (gr  : gpu_array u64 (nblk * nthr))
+  (v1: erased (seq u64) { Seq.length v1 == Kernel.rows * Kernel.shared })
+  (v2: erased (seq u64) { Seq.length v2 == Kernel.shared * Kernel.columns })
+  requires gpu_pts_to_array gr 's **
+           gpu_pts_to_array ga1 v1 **
+           gpu_pts_to_array ga2 v2
+  ensures  bigstar 0 (nblk * nthr) (fun i ->
+             Kernel.kpre Kernel.rows Kernel.shared Kernel.columns ga1 ga2 gr #v1 #v2 (nblk * nthr) (Kernel.tid_to_idx i))
+{
+  // Sharing the input matrices (splitting permissions)
+  fold Defs.gpu_pts_to_matrix Kernel.rows   Kernel.shared  ga1 1 v1;
+  fold Defs.gpu_pts_to_matrix Kernel.shared Kernel.columns ga2 1 v2;
+  Defs.gpu_matrix_share_underspec #_ #1 Kernel.rows   Kernel.shared  ga1 (nblk * nthr) v1;
+  Defs.gpu_matrix_share_underspec #_ #2 Kernel.shared Kernel.columns ga2 (nblk * nthr) v2;
+
+  // Sharing the output matrix (splitting each cell)
+  gpu_pts_to_ref gr; (* obtain length v == (nblk * nthr) *)
+  gpu_array_slice_1 #4 gr;
+
+  // Join resources into a single bigstar
+  bigstar_zip #1 #2 #3 0 (nblk * nthr) _ _;
+  bigstar_zip #3 #4 #0 0 (nblk * nthr) _ _;
+
+  // Rewrite inside the bigstar
+  ghost
+  fn aux (i:nat{0 <= i /\ i < (nblk * nthr)})
+    requires
+      Defs.gpu_pts_to_matrix Kernel.rows   Kernel.shared  ga1 (nblk * nthr) v1 **
+      Defs.gpu_pts_to_matrix Kernel.shared Kernel.columns ga2 (nblk * nthr) v2 **
+      gpu_pts_to_array_slice gr i (i + 1) seq!['s `Seq.index` i]
+    ensures
+      Kernel.kpre Kernel.rows Kernel.shared Kernel.columns ga1 ga2 gr #v1 #v2 (nblk * nthr) i
+  {
+    fold gpu_pts_to_array1 gr i;
+    ()
+  };
+  bigstar_map #_ #_ #0 #(nblk * nthr) aux;
+  bigstar_permute #0 #0 #(nblk * nthr) #_ (Kernel.permute());
+  ghost fn rewrite_permute_to_fn (i: nat {0 <= i /\ i < (nblk * nthr)})
+    requires Kernel.kpre Kernel.rows Kernel.shared Kernel.columns ga1 ga2 gr #v1 #v2 (nblk * nthr) ((Kernel.permute()).f i)
+    ensures  Kernel.kpre Kernel.rows Kernel.shared Kernel.columns ga1 ga2 gr #v1 #v2 (nblk * nthr) (Kernel.tid_to_idx i)
+  {
+    ()
+  };
+  bigstar_map #0 #0 #0 #(nblk * nthr) (fun i -> rewrite_permute_to_fn i);
+  ()
+}
+
+ghost
+fn breakdown
+  (nblk: sz { nblk == SZ.(Kernel.rows_tile *^ Kernel.columns_tile) })
+  (nthr: sz { nthr == SZ.(Kernel.bdim *^ Kernel.bdim) })
+  (ga1 : gpu_array u64 (Kernel.rows * Kernel.shared))
+  (ga2 : gpu_array u64 (Kernel.shared * Kernel.columns))
+  (gr  : gpu_array u64 (nblk * nthr))
+  (v1: erased (seq u64) { Seq.length v1 == Kernel.rows * Kernel.shared })
+  (v2: erased (seq u64) { Seq.length v2 == Kernel.shared * Kernel.columns })
+  requires bigstar 0 (nblk * nthr) (fun i ->
+             Kernel.kpost Kernel.rows Kernel.shared Kernel.columns ga1 ga2 gr #v1 #v2 (nblk * nthr) (Kernel.tid_to_idx i))
+  ensures  (exists* vr. gpu_pts_to_array gr vr) **
+           gpu_pts_to_array ga1 v1 **
+           gpu_pts_to_array ga2 v2
+{
+  let perm = perm_inv (Kernel.permute());
+  bigstar_permute #0 #0 #(nblk * nthr) #_ perm;
+  ghost fn rewrite_permute_to_fn (i: nat {0 <= i /\ i < (nblk * nthr)})
+    requires Kernel.kpost Kernel.rows Kernel.shared Kernel.columns ga1 ga2 gr #v1 #v2 (nblk * nthr) (perm.f (Kernel.tid_to_idx i))
+    ensures  Kernel.kpost Kernel.rows Kernel.shared Kernel.columns ga1 ga2 gr #v1 #v2 (nblk * nthr) i
+  {
+    let once: (j: nat{ 0 <= j /\ j < (nblk * nthr) }) = Kernel.tid_to_idx i;
+    let once': (j: nat{ 0 <= j /\ j < (nblk * nthr) }) = perm.g i;
+    assert (pure (once' == once));
+    perm.proof once i;
+    // f x == y <==> g y == x
+    let double: (j: nat{ 0 <= j /\ j < (nblk * nthr) }) = perm.f once;
+    assert (pure (double == i));
+    rewrite (gpu_pts_to_array1 gr (perm.f (Kernel.tid_to_idx i)))
+         as (gpu_pts_to_array1 gr i);
+    ()
+  };
+  bigstar_map #0 #0 #0 #(nblk * nthr) (fun i -> rewrite_permute_to_fn i);
+
+  // Join resources into a single bigstar
+  bigstar_unzip #3 #4 #0 0 (nblk * nthr) _ _;
+  bigstar_unzip #1 #2 #3 0 (nblk * nthr) _ _;
+
+  gpu_array_unslice_1_underspec #4 gr #1.0R;
+
+  // Unsharing the input matrices (gathering permissions)
+  Defs.gpu_matrix_unshare_underspec #_ #1 Kernel.rows   Kernel.shared  ga1 (nblk * nthr) v1;
+  Defs.gpu_matrix_unshare_underspec #_ #2 Kernel.shared Kernel.columns ga2 (nblk * nthr) v2;
+  unfold Defs.gpu_pts_to_matrix Kernel.rows   Kernel.shared  ga1 1 v1;
+  unfold Defs.gpu_pts_to_matrix Kernel.shared Kernel.columns ga2 1 v2;
+
+  ()
+}
+
+fn main
+  (a1 a2: array u64)
+  (v1: erased (seq u64) { Seq.length v1 == Kernel.rows * Kernel.shared })
+  (v2: erased (seq u64) { Seq.length v2 == Kernel.shared * Kernel.columns })
+  requires cpu ** A.pts_to a1 v1 ** A.pts_to a2 v2
+  returns  ar: array u64
+  ensures  cpu ** A.pts_to a1 v1 ** A.pts_to a2 v2 ** (exists* vr. A.pts_to ar vr)
+{
+  open FStar.SizeT;
+  let nblk = Kernel.rows_tile *^ Kernel.columns_tile;
+  let nthr = Kernel.bdim *^ Kernel.bdim;
+  let size = nblk *^ nthr;
+  let ar = Pulse.Lib.Array.alloc 0UL size;
+
+  let ga1 = gpu_array_alloc #u64 (Kernel.rows *^ Kernel.shared);
+  let ga2 = gpu_array_alloc #u64 (Kernel.shared *^ Kernel.columns);
+
+  GPU.Array.gpu_memcpy_host_to_device a1 ga1 (Kernel.rows *^ Kernel.shared);
+  GPU.Array.gpu_memcpy_host_to_device a2 ga2 (Kernel.shared *^ Kernel.columns);
+
+  let gr = gpu_array_alloc #u64 size;
+
+  setup nblk nthr ga1 ga2 gr v1 v2;
+
+  let smem_sz = 2sz *^ nthr;
+  launch_kernel_n_m_sync #0
+    nblk
+    nthr
+    #(fun (tid: nat {0 <= tid /\ tid < (nblk * nthr)} ) -> Kernel.kpre Kernel.rows Kernel.shared Kernel.columns ga1 ga2 gr #v1 #v2 (nblk * nthr) (Kernel.tid_to_idx tid))
+    #(fun (tid: nat {0 <= tid /\ tid < (nblk * nthr)} ) -> Kernel.kpost Kernel.rows Kernel.shared Kernel.columns ga1 ga2 gr #v1 #v2 (nblk * nthr) (Kernel.tid_to_idx tid))
+    u64
+    smem_sz
+    #(Barrier.shared_pre nthr 0)
+    #(Barrier.shared_pre nthr (2 * Kernel.columns_tile))
+    (Barrier.block_setup_ghost nthr smem_sz)
+    (fun ar etid -> Kernel.kernel ga1 ga2 gr #v1 #v2 (hide nblk) (hide nthr) smem_sz ar etid);
+
+  breakdown nblk nthr ga1 ga2 gr v1 v2;
+
+  GPU.Array.gpu_memcpy_device_to_host ar gr size;
+
+  gpu_array_free ga1;
+  gpu_array_free ga2;
+  gpu_array_free gr;
+
+  ar
+}
