src/examples/matmul-tile/GPU.MatMulTile.Kernel.fst
@@ -1,0 +1,290 @@
+module GPU.MatMulTile.Kernel
+
+#lang-pulse
+
+open GPU
+open GPU.Barrier.RPM
+open FStar.SizeT
+module SZ = FStar.SizeT
+
+#set-options "--z3rlimit 10"
+#push-options "--fuel 6 --ifuel 6"
+
+// #push-options "--print_implicits --print_bound_var_types"
+// #push-options "--debug SMTFail"
+
+let lemma_pos_times_pos (a b: pos)
+  : Lemma (a * b > 0) = ()
+
+let lemma_nat_times_nat (a b: nat)
+  : Lemma (a * b >= 0) = ()
+
+fn calc_idxs
+  (nblk : erased sz { SZ.v nblk == SZ.v SZ.(rows_tile *^ columns_tile) })
+  (nthr : erased sz { SZ.v nthr == SZ.v SZ.(bdim *^ bdim) })
+  (etid : tid_t { gdim_x etid == nthr /\ bdim_x etid == nblk })
+  requires thread_id etid
+  returns  idxs: (SZ.t & SZ.t & SZ.t)
+  ensures  thread_id etid ** (pure (SZ.v idxs._1 == (tid_to_idx (thread_index etid)) /\ SZ.v idxs._2 < rows /\ SZ.v idxs._3 < columns))
+{
+  let tid = thread_idx_x () <: u32;
+  let tid : sz = SZ.uint32_to_sizet tid;
+  let trow = SZ.div tid bdim;
+  let tcol = SZ.rem tid bdim;
+  assert (pure (SZ.v trow <= SZ.v bdim - 1 /\ SZ.v tcol <= SZ.v bdim - 1));
+
+  let bid = block_idx_x () <: u32;
+  let bid : sz = SZ.uint32_to_sizet bid;
+  let brow = SZ.div bid columns_tile;
+  let bcol = SZ.rem bid columns_tile;
+  assert (pure (SZ.v brow <= SZ.v rows_tile - 1 /\ SZ.v bcol <= SZ.v columns_tile - 1));
+
+  let brow_idx = brow *^ bdim *^ columns_tile *^ bdim;
+  let trow_idx = trow *^ bdim *^ columns_tile;
+  let bcol_idx = bcol *^ bdim;
+  assert (pure (SZ.v brow_idx <= (rows_tile - 1) * bdim * columns_tile * bdim));
+  assert (pure (SZ.v trow_idx <= (bdim - 1) * columns_tile * bdim));
+  assert (pure (SZ.v bcol_idx <= (columns_tile - 1) * bdim));
+
+  assert (pure (SZ.v bcol_idx + SZ.v tcol < columns_tile * bdim));
+  let bcol_tcol_idx = bcol_idx +^ tcol;
+
+  assert (pure (SZ.v trow_idx + SZ.v bcol_tcol_idx < bdim * columns_tile * bdim));
+  let trow_bcol_tcol_idx = trow_idx +^ bcol_tcol_idx;
+
+  assert (pure (SZ.v brow_idx + SZ.v trow_bcol_tcol_idx < rows_tile * bdim * columns_tile * bdim));
+  let idx : sz = brow_idx +^ trow_bcol_tcol_idx;
+
+  lemma_nat_times_nat (SZ.v bid) (SZ.v nthr);
+  FStar.Math.Lemmas.lemma_mult_le_right (SZ.v nthr) (SZ.v bid) (SZ.v nblk - 1);
+  assert (pure (SZ.v bid * SZ.v nthr <= (SZ.v nblk - 1) * SZ.v nthr));
+  FStar.Math.Lemmas.distributivity_sub_left (SZ.v nblk) 1 (SZ.v nthr);
+  assume_ (pure (SZ.v idx == tid_to_idx (SZ.v bid * SZ.v nthr + SZ.v tid))); // TODO
+
+  assert (pure (SZ.v rows_tile == 32 /\ SZ.v columns_tile == 32 /\ SZ.v bdim == 32));
+
+  let brow_bdim = brow *^ bdim;
+  let bcol_bdim = bcol *^ bdim;
+  let row : sz = brow_bdim +^ trow;
+  let col : sz = bcol_bdim +^ tcol;
+
+  FStar.Math.Lemmas.lemma_mult_le_right (SZ.v bdim) (SZ.v brow) (SZ.v rows_tile - 1);
+  FStar.Math.Lemmas.lemma_mult_le_right (SZ.v bdim) (SZ.v bcol) (SZ.v columns_tile - 1);
+  assert (pure (SZ.v row <= (SZ.v rows_tile - 1) * SZ.v bdim + (SZ.v bdim - 1)));
+  FStar.Math.Lemmas.distributivity_sub_left (SZ.v rows_tile) 1 (SZ.v bdim);
+  assert (pure ((SZ.v rows_tile - 1) * SZ.v bdim + (SZ.v bdim - 1) == SZ.v rows - SZ.v bdim + SZ.v bdim - 1));
+  
+  assert (pure (SZ.v col <= (SZ.v columns_tile - 1) * SZ.v bdim + (SZ.v bdim - 1)));
+  FStar.Math.Lemmas.distributivity_sub_left (SZ.v columns_tile) 1 (SZ.v bdim);
+  assert (pure ((SZ.v columns_tile - 1) * SZ.v bdim + (SZ.v bdim - 1) == SZ.v columns - 1));
+  assert (pure (SZ.v row < SZ.v rows /\ SZ.v col < SZ.v columns));
+
+  Mktuple3 idx row col
+}
+
+let sz_mult (x y: SZ.t) : Pure SZ.t
+  (requires (SZ.fits (SZ.v x * SZ.v y)))
+  (ensures (fun z -> SZ.v z == SZ.v x * SZ.v y)) = SZ.mul x y
+
+let lemma_div_pos (a: real) (i: int)
+  : Lemma (requires (a >. 0.0R /\ i > 0))
+          (ensures (a /. Real.of_int i >. 0.0R)) = ()
+
+let lemma_mod_lt (a : nat) (b : pos)
+  : Lemma (a % b <= b - 1) = ()
+
+let lemma_div_lt (a : nat) (b c: pos)
+  : Lemma (requires (a < c * b))
+          (ensures  (a / b < c)) = ()
+
+fn inner_loop
+  (vv : sz{SZ.v vv <= SZ.v bdim - 1})
+  (ga1_iidx : sz{SZ.v ga1_iidx <= (SZ.v bdim - 1) * SZ.v bdim})
+  (ga2_iidx : sz{SZ.v ga2_iidx <= SZ.v bdim - 1})
+  (nthr : erased nat{nthr == SZ.v SZ.(bdim *^ bdim)})
+  (ar : gpu_array u64 (2 * nthr))
+  (it: erased nat{it % 2 <> 0})
+  (tid: erased nat{0 <= tid /\ tid < nthr})
+  (sum : ref u64)
+  requires gpu
+        ** (exists* sumv. pts_to sum sumv)
+        ** bigstar 0 nthr (Barrier.barrier_mm nthr ar it tid)
+  ensures  gpu
+        ** (exists* sumv. pts_to sum sumv)
+        ** bigstar 0 nthr (Barrier.barrier_mm nthr ar it tid)
+{
+  FStar.Math.Lemmas.lemma_mult_le_right (SZ.v bdim) (SZ.v vv) (SZ.v bdim - 1);
+  
+  let ga1_idx = ga1_iidx +^ vv;
+  assert (pure (SZ.v ga1_idx < nthr));
+
+  let ga2_idx = ga2_iidx +^ (vv *^ bdim);
+  assert (pure (SZ.v ga2_idx < nthr));
+
+  bigstar_extract #0 0 nthr _ ga1_idx;
+  unfold Barrier.barrier_mm nthr ar it tid ga1_idx;
+  let ga1_val = gpu_array_read #_ #_ #(2 * ga1_idx) #(2 * ga1_idx + 2) ar #(1.0R /. Real.of_int nthr) (2sz *^ ga1_idx);
+  fold Barrier.barrier_mm nthr ar it tid ga1_idx;
+  bigstar_compose #0 0 nthr _ ga1_idx;
+
+  bigstar_extract #0 0 nthr _ ga2_idx;
+  unfold Barrier.barrier_mm nthr ar it tid ga2_idx;
+  let ga2_val = gpu_array_read #_ #_ #(2 * ga2_idx) #(2 * ga2_idx + 2) ar #(1.0R /. Real.of_int nthr) (2sz *^ ga2_idx +^ 1sz);
+  fold Barrier.barrier_mm nthr ar it tid ga2_idx;
+  bigstar_compose #0 0 nthr _ ga2_idx;
+
+  let s = !sum;
+  sum := U64.add_mod (U64.mul_mod ga1_val ga2_val) s;
+}
+
+fn outer_loop
+  (iv: sz{SZ.v iv <= shared_tile - 1})
+  (nthr: erased nat{nthr == SZ.v SZ.(bdim *^ bdim)})
+  (smem_sz: erased nat{smem_sz == 2 * nthr})
+  (ar: gpu_array u64 smem_sz)
+  (tid: erased nat{0 <= tid /\ tid < nthr})
+  (tcol: sz{SZ.v tcol < SZ.v bdim})
+  (trow: sz{SZ.v trow < SZ.v bdim})
+  (sum: ref u64)
+  requires gpu
+       ** (exists* sumv. pts_to sum sumv)
+       ** (exists* s. gpu_pts_to_array_slice ar (2 * tid) (2 * tid + 2) s)
+       ** mbarrier_tok nthr (Barrier.barrier_mm nthr ar) (2*iv) tid
+  ensures gpu
+       ** (exists* sumv. pts_to sum sumv)
+       ** (exists* s. gpu_pts_to_array_slice ar (2 * tid) (2 * tid + 2) s)
+       ** mbarrier_tok nthr (Barrier.barrier_mm nthr ar) (2*iv + 2) tid
+{
+  lemma_div_pos 1.0R nthr; // 1.0R /. Real.of_int nthr >. 0.0R
+
+  FStar.Math.Lemmas.cancel_mul_mod (SZ.v iv) 2;
+  FStar.Math.Lemmas.lemma_mod_plus 1 (SZ.v iv) 2;
+  assert (pure ((SZ.v iv * 2) % 2 == 0 /\ (1 + SZ.v iv * 2) % 2 <> 0));
+
+  // Share smem permission with all threads
+  gpu_slice_share_underspec #0 #u64 #smem_sz ar #1.0R (2 * tid) (2 * tid + 2) nthr;
+  bigstar_map #0 #0 #0 #nthr #_ #_ (Barrier.fold_barrier_mm_even nthr smem_sz ar (2*iv) tid);
+  mbarrier_wait #nthr #(Barrier.barrier_mm nthr ar) #(2 * SZ.v iv) #tid;
+  bigstar_map #0 #0 #0 #nthr #_ #_ (fun from -> Barrier.transfer_barrier_mm nthr smem_sz ar (2*iv) from tid);
+
+  // Do stuff
+  let ga1_iidx = trow *^ bdim;
+  let ga2_iidx = tcol;
+
+  let mut j = 0sz;
+  while (let vv = !j; (vv <^ bdim))
+    invariant b.
+      exists* vv.
+      pure (b == (SZ.v vv < bdim) /\ SZ.v vv <= bdim /\ SZ.v vv >= 0) **
+      pts_to j vv **
+      gpu
+      ** (exists* sumv. pts_to sum sumv)
+      ** bigstar 0 nthr (Barrier.barrier_mm nthr ar (2*iv + 1) tid)
+  {
+    let vv = !j;
+    j := SZ.add vv 1sz;
+
+    inner_loop vv ga1_iidx ga2_iidx nthr ar (2*iv + 1) tid sum;
+
+    ()
+  };
+
+  // Send smem permission back to single thread
+  mbarrier_wait #nthr #(Barrier.barrier_mm nthr ar) #(2 * SZ.v iv + 1) #tid;
+  bigstar_map #0 #0 #0 #nthr #_ #_ (fun from -> Barrier.transfer_barrier_mm nthr smem_sz ar (2*iv + 1) from tid);
+  bigstar_map #0 #0 #0 #nthr #_ #_ (Barrier.unfold_barrier_mm_even nthr smem_sz ar (2*iv + 2) tid);
+  gpu_slice_gather_underspec #0 #u64 #smem_sz ar #1.0R (2 * tid) (2 * tid + 2) nthr;
+}
+
+[@@CPrologue "__global__"]
+fn kernel
+  // (rows: nat) (shared: nat { shared < pow2 16 }) (columns: nat)
+  (ga1 : gpu_array u64 (rows * shared))
+  (ga2 : gpu_array u64 (shared * columns))
+  (r : gpu_array u64 (rows * columns))
+  (#s1: erased (seq u64) {Seq.length s1 == rows * shared})
+  (#s2: erased (seq u64) {Seq.length s2 == shared * columns})
+  (nblk : erased sz { SZ.v nblk == SZ.v SZ.(rows_tile *^ columns_tile) })
+  (nthr : erased sz { SZ.v nthr == SZ.v SZ.(bdim *^ bdim) })
+  (smem_sz : sz { SZ.v smem_sz == 2 * SZ.v nthr })
+  (ar: gpu_array u64 smem_sz)
+  (etid : tid_t { gdim_x etid == nthr /\ bdim_x etid == nblk })
+  requires gpu
+    ** thread_id etid
+    ** Barrier.shared_pre nthr 0 ar (SZ.v (bidx_x etid)) (SZ.v (tidx_x etid))
+    ** kpre rows shared columns ga1 ga2 r #s1 #s2 (SZ.v nblk * SZ.v nthr) (tid_to_idx (thread_index etid))
+  ensures  gpu
+    ** thread_id etid
+    ** Barrier.shared_pre nthr (2 * shared_tile) ar (SZ.v (bidx_x etid)) (SZ.v (tidx_x etid))
+    ** kpost rows shared columns ga1 ga2 r #s1 #s2 (SZ.v nblk * SZ.v nthr) (tid_to_idx (thread_index etid))
+{
+
+  let idxs = calc_idxs nblk nthr etid;
+  let idx = idxs._1;
+  let row = idxs._2;
+  let col = idxs._3;
+
+  let tid = thread_idx_x () <: u32;
+  let tid : sz = SZ.uint32_to_sizet tid;
+  assert (pure (SZ.v tid < SZ.v bdim * SZ.v bdim));
+  let trow : sz = SZ.div tid bdim;
+  let tcol : sz = SZ.rem tid bdim;
+  // lemmas
+  FStar.Math.Lemmas.euclidean_division_definition (SZ.v tid) (SZ.v bdim);
+  lemma_div_lt (SZ.v tid) (SZ.v bdim) (SZ.v bdim);
+  lemma_mod_lt (SZ.v tid) (SZ.v bdim);
+  assert (pure (SZ.v trow < SZ.v bdim /\ SZ.v tcol < SZ.v bdim));
+
+  let smem_idx1 = 2sz *^ tid;
+  let smem_idx2 = 2sz *^ tid +^ 1sz;
+
+  let mut i = 0sz;
+  let mut sum = 0UL;
+
+  unfold Barrier.shared_pre;
+  while (let iv = !i; (iv <^ shared_tile))
+     invariant b.
+       exists* iv.
+       pure (b == (SZ.v iv < shared_tile) /\ SZ.v iv <= shared_tile /\ SZ.v iv >= 0) **
+       pts_to i iv **
+       gpu
+       ** (exists* sumv. pts_to sum sumv)
+       ** Impure.gpu_pts_to_matrix #u64 rows shared ga1 (SZ.v nblk * SZ.v nthr) s1
+       ** Impure.gpu_pts_to_matrix #u64 shared columns ga2 (SZ.v nblk * SZ.v nthr) s2
+       ** (exists* s. gpu_pts_to_array_slice ar (2 * tid) (2 * tid + 2) s)
+       ** mbarrier_tok (SZ.v nthr) (Barrier.barrier_mm (SZ.v nthr) ar) (2*iv) tid
+  {
+    let iv = !i;
+    i := SZ.add iv 1sz;
+    FStar.Math.Lemmas.cancel_mul_mod (SZ.v iv) 2;
+
+    FStar.Math.Lemmas.lemma_mult_le_right (SZ.v bdim) (SZ.v iv) (SZ.v shared_tile - 1);
+    assert (pure (SZ.v iv * SZ.v bdim <= (SZ.v shared_tile - 1) * SZ.v bdim));
+    assert (pure (SZ.v shared_tile == 32 /\ SZ.v bdim == 32));
+    SZ.fits_at_least_16 (SZ.v iv * SZ.v bdim);
+    
+    let v_bdim = SZ.mul iv bdim;
+
+    assert (pure (SZ.v v_bdim + SZ.v tcol < shared /\ SZ.v v_bdim + SZ.v trow < shared));
+    SZ.fits_at_least_16 (SZ.v v_bdim + SZ.v tcol);
+    SZ.fits_at_least_16 (SZ.v v_bdim + SZ.v trow);
+    assert (pure (SZ.v row < SZ.v rows /\ SZ.v col < SZ.v columns));
+
+    let v1 = Impure.gpu_matrix_read #_ #rows #shared ga1 #(SZ.v nblk * SZ.v nthr) #s1 row (v_bdim +^ tcol);
+    let v2 = Impure.gpu_matrix_read #_ #shared #columns ga2 #(SZ.v nblk * SZ.v nthr) #s2 (v_bdim +^ trow) col;
+    
+    gpu_array_write #u64 #smem_sz #(SZ.v smem_idx1) #(SZ.v smem_idx1 + 2) ar smem_idx1 v1;
+    gpu_array_write #u64 #smem_sz #(SZ.v smem_idx1) #(SZ.v smem_idx1 + 2) ar smem_idx2 v2;
+
+    outer_loop iv (SZ.v nthr) (SZ.v smem_sz) ar (SZ.v tid) tcol trow sum;
+    ()
+  };
+  fold Barrier.shared_pre nthr (2 * shared_tile) ar (SZ.v (bidx_x etid)) (SZ.v (tidx_x etid));
+
+  let s = !sum;
+  unfold gpu_pts_to_array1 r (tid_to_idx (thread_index etid));
+  gpu_array_write #u64 #(rows * columns) #(SZ.v idx) #(SZ.v idx + 1) r idx s;
+  fold gpu_pts_to_array1 r (tid_to_idx (thread_index etid));
+
+  ()
+}
