src/examples/matmul-tile/GPU.MatMulTile.Kernel.fsti
@@ -1,0 +1,115 @@
+module GPU.MatMulTile.Kernel
+
+#lang-pulse
+
+#push-options "--fuel 1 --ifuel 1"
+
+open GPU
+
+module Impure = GPU.MatMul.Impure
+module Pure = GPU.MatMul.Pure
+module Barrier = GPU.MatMulTile.Barrier
+module SZ = FStar.SizeT
+module U64 = FStar.UInt64
+module Layout4 = GPU.MatMulTile.Layout4
+
+[@@pulse_unfold]
+let kpre_pair (rows shared columns: nat)
+  (ga1: gpu_array u64 (rows * shared))
+  (ga2: gpu_array u64 (shared * columns))
+  (#s1: erased (seq u64))
+  (#s2: erased (seq u64))
+  (nthr: erased nat { nthr > 0 })
+  : slprop
+  =
+  Impure.gpu_pts_to_matrix rows shared ga1 nthr s1
+  ** Impure.gpu_pts_to_matrix shared columns ga2 nthr s2
+
+[@@pulse_unfold]
+let kpre (rows shared columns: nat)
+  (ga1: gpu_array u64 (rows * shared))
+  (ga2: gpu_array u64 (shared * columns))
+  (r: gpu_array u64 (rows * columns))
+  (#s1: erased (seq u64) )
+  (#s2: erased (seq u64))
+  (nthr: erased nat { nthr > 0 })
+  (tid : nat{ tid < rows * columns})
+  : slprop
+  =
+  kpre_pair rows shared columns ga1 ga2 #s1 #s2 nthr
+  ** gpu_pts_to_array1 r tid
+
+[@@pulse_unfold]
+let kpost (rows shared columns: nat)
+  (ga1: gpu_array u64 (rows * shared))
+  (ga2: gpu_array u64 (shared * columns))
+  (r: gpu_array u64 (rows * columns))
+  (#s1: erased (seq u64) {Seq.length s1 == rows * shared})
+  (#s2: erased (seq u64) {Seq.length s2 == shared * columns})
+  (nthr: erased nat { nthr > 0 })
+  (tid : nat {  tid < rows * columns })
+  : slprop
+  =
+  Impure.gpu_pts_to_matrix rows shared ga1 nthr s1
+  ** Impure.gpu_pts_to_matrix shared columns ga2 nthr s2
+  ** gpu_pts_to_array1 r tid
+  // ** (exists* s. gpu_pts_to_array_slice r tid (tid+1) s)
+
+
+// TODO: un-hardcode
+[@@CPrologue "const"]
+inline_for_extraction
+let bdim : sz = 32sz // rows/columns of tiles
+
+[@@CPrologue "const"]
+inline_for_extraction
+let rows_tile : sz = 32sz // rows of ga1/r (in tiles)
+
+[@@CPrologue "const"]
+inline_for_extraction
+let shared_tile : sz = rows_tile // columns of ga1, rows of ga2 (in tiles)
+
+[@@CPrologue "const"]
+inline_for_extraction
+let columns_tile : sz = rows_tile // columns of ga2/r (in tiles)
+
+[@@CPrologue "const"]
+inline_for_extraction
+let rows : sz = SZ.(rows_tile *^ bdim) // rows of ga1/r
+
+[@@CPrologue "const"]
+inline_for_extraction
+let shared : sz = SZ.(shared_tile *^ bdim) // columns of ga1, rows of ga2
+
+[@@CPrologue "const"]
+inline_for_extraction
+let columns : sz = SZ.(columns_tile *^ bdim) // columns of ga2/r
+
+let permute(): GTot (permutation (i: nat { 0 <= i /\ i < SZ.(rows_tile *^ columns_tile) * SZ.(bdim *^ bdim) })) = Layout4.titi_permutation bdim bdim rows_tile columns_tile
+
+let tid_to_idx (tid: nat { 0 <= tid /\ tid < rows * columns })
+  : GTot (tid: nat { 0 <= tid /\ tid < rows * columns })
+  = assert (SZ.(rows_tile *^ columns_tile) * SZ.(bdim *^ bdim) == rows * columns);
+    (permute()).f tid
+
+[@@CPrologue "__global__"]
+fn kernel
+  // (rows: nat) (shared: nat { shared < pow2 16 }) (columns: nat)
+  (ga1 : gpu_array u64 (rows * shared))
+  (ga2 : gpu_array u64 (shared * columns))
+  (r : gpu_array u64 (rows * columns))
+  (#s1: erased (seq u64) {Seq.length s1 == rows * shared})
+  (#s2: erased (seq u64) {Seq.length s2 == shared * columns})
+  (nblk : erased sz { SZ.v nblk == SZ.v SZ.(rows_tile *^ columns_tile) })
+  (nthr : erased sz { SZ.v nthr == SZ.v SZ.(bdim *^ bdim) })
+  (smem_sz : sz { SZ.v smem_sz == 2 * SZ.v nthr })
+  (ar: gpu_array u64 smem_sz)
+  (etid : tid_t { gdim_x etid == nthr /\ bdim_x etid == nblk })
+  requires gpu
+    ** thread_id etid
+    ** Barrier.shared_pre nthr 0 ar (SZ.v (bidx_x etid)) (SZ.v (tidx_x etid))
+    ** kpre rows shared columns ga1 ga2 r #s1 #s2 (SZ.v nblk * SZ.v nthr) (tid_to_idx (thread_index etid))
+  ensures  gpu
+    ** thread_id etid
+    ** Barrier.shared_pre nthr (2 * columns_tile) ar (SZ.v (bidx_x etid)) (SZ.v (tidx_x etid))
+    ** kpost rows shared columns ga1 ga2 r #s1 #s2 (SZ.v nblk * SZ.v nthr) (tid_to_idx (thread_index etid))
